concurrency/concurrent_machine.v
@@ -25,7 +25,6 @@ Require Import concurrency.safety.
 Require Import concurrency.coinductive_safety.
 
 
-
 Notation EXIT :=
   (EF_external "EXIT" (mksignature (AST.Tint::nil) None)).
 
@@ -147,7 +146,7 @@ Module Type ConcurrentMachineSig.
 
   (*Parameter initial_machine: C -> thread_pool.*)
 
-  Parameter init_mach : option RES.res  -> G -> val -> list val -> option thread_pool.
+  Parameter init_mach : option RES.res  -> G -> mem -> val -> list val -> option (thread_pool * option mem).
 
 End ConcurrentMachineSig.
 
@@ -190,62 +189,62 @@ Module CoarseMachine (SCH:Scheduler)(SIG : ConcurrentMachineSig with Module Thre
      running. (This keeps the invariant that at most one thread is not
      at_external) *)
 
-  Inductive start_thread' genv: forall {tid0} {ms:machine_state},
-      containsThread ms tid0 -> machine_state -> Prop:=
-  | StartThread: forall tid0 ms ms' c_new vf arg
+  Inductive start_thread' genv: forall  (m: mem) {tid0} {ms:machine_state},
+      containsThread ms tid0 -> machine_state -> mem -> Prop:=
+  | StartThread: forall m tid0 ms ms' c_new om vf arg
                     (ctn: containsThread ms tid0)
                     (Hcode: getThreadC ctn = Kinit vf arg)
                     (Hinitial: initial_core Sem (tid2nat tid0)
-                                            genv vf (arg::nil) = Some c_new)
+                                            genv m vf (arg::nil) = Some (c_new, om))
                     (Hinv: invariant ms)
                     (Hms': updThreadC ctn (Krun c_new)  = ms'),
-      start_thread' genv ctn ms'.
-  Definition start_thread genv: forall {tid0 ms},
-      containsThread ms tid0 -> machine_state -> Prop:=
+      start_thread' genv m ctn ms' (option_proj m om).
+  Definition start_thread genv: forall (m: mem) {tid0 ms},
+      containsThread ms tid0 -> machine_state -> mem -> Prop:=
     @start_thread' genv.
-  Inductive resume_thread': forall {tid0} {ms:machine_state},
+  Inductive resume_thread' ge: forall (m: mem) {tid0} {ms:machine_state},
       containsThread ms tid0 -> machine_state -> Prop:=
-  | ResumeThread: forall tid0 ms ms' c c' X
+  | ResumeThread: forall m tid0 ms ms' c c' X
                     (ctn: containsThread ms tid0)
-                    (Hat_external: at_external Sem c = Some X)
-                    (Hafter_external: after_external Sem None c = Some c')
+                    (Hat_external: at_external Sem ge c m = Some X)
+                    (Hafter_external: after_external Sem ge None c = Some c')
                     (Hcode: getThreadC ctn = Kresume c Vundef)
                     (Hinv: invariant ms)
                     (Hms': updThreadC ctn (Krun c')  = ms'),
-      resume_thread' ctn ms'.
-  Definition resume_thread: forall {tid0 ms},
+      resume_thread' ge m ctn ms'.
+  Definition resume_thread genv: forall m {tid0 ms},
       containsThread ms tid0 -> machine_state -> Prop:=
-    @resume_thread'.
+    @resume_thread' genv.
 
-  Inductive suspend_thread': forall {tid0} {ms:machine_state},
+  Inductive suspend_thread' ge: forall (m: mem) {tid0} {ms:machine_state},
       containsThread ms tid0 -> machine_state -> Prop:=
-  | SuspendThread: forall tid0 ms ms' c X
+  | SuspendThread: forall m tid0 ms ms' c X
                      (ctn: containsThread ms tid0)
                      (Hcode: getThreadC ctn = Krun c)
-                     (Hat_external: at_external Sem c = Some X)
+                     (Hat_external: at_external Sem ge c m = Some X)
                      (Hinv: invariant ms)
                      (Hms': updThreadC ctn (Kblocked c) = ms'),
-      suspend_thread' ctn ms'.
-  Definition suspend_thread : forall {tid0 ms},
+      suspend_thread' ge m ctn ms'.
+  Definition suspend_thread ge: forall m {tid0 ms},
       containsThread ms tid0 -> machine_state -> Prop:=
-    @suspend_thread'.
+    @suspend_thread' ge.
 
   Inductive machine_step {genv:G}:
     Sch -> event_trace -> machine_state -> mem -> Sch ->
     event_trace -> machine_state -> mem -> Prop :=
   | start_step:
-      forall tid U ms ms' m
+      forall tid U ms ms' m m'
         (HschedN: schedPeek U = Some tid)
         (Htid: containsThread ms tid)
         (Hcmpt: mem_compatible ms m)
-        (Htstep: start_thread genv Htid ms'),
-        machine_step U [::] ms m U [::] ms' m
+        (Htstep: start_thread genv m Htid ms' m'),
+        machine_step U [::] ms m U [::] ms' m'
   | resume_step:
       forall tid U ms ms' m
         (HschedN: schedPeek U = Some tid)
         (Htid: containsThread ms tid)
         (Hcmpt: mem_compatible ms m)
-        (Htstep: resume_thread Htid ms'),
+        (Htstep: resume_thread genv m Htid ms'),
         machine_step U [::] ms m U [::] ms' m
   | thread_step:
       forall tid U ms ms' m m' ev
@@ -260,7 +259,7 @@ Module CoarseMachine (SCH:Scheduler)(SIG : ConcurrentMachineSig with Module Thre
         (HschedS: schedSkip U = U')        (*Schedule Forward*)
         (Htid: containsThread ms tid)
         (Hcmpt: mem_compatible ms m)
-        (Htstep:suspend_thread Htid ms'),
+        (Htstep:suspend_thread genv m Htid ms'),
         machine_step U [::] ms m U' [::] ms' m
   | sync_step:
       forall tid U U' ms ms' m m' ev
@@ -307,18 +306,18 @@ Module CoarseMachine (SCH:Scheduler)(SIG : ConcurrentMachineSig with Module Thre
   Inductive external_step  {genv:G}:
     Sch -> event_trace -> machine_state -> mem -> Sch ->
     event_trace -> machine_state -> mem -> Prop :=
-  | start_state': forall tid U ms ms' m
+  | start_state': forall tid U ms ms' m m'
         (HschedN: schedPeek U = Some tid)
         (Htid: containsThread ms tid)
         (Hcmpt: mem_compatible ms m)
-        (Htstep: start_thread genv Htid ms'),
-        external_step U [::] ms m U [::] ms' m
+        (Htstep: start_thread genv m Htid ms' m'),
+        external_step U [::] ms m U [::] ms' m'
   | resume_step':
       forall tid U ms ms' m
         (HschedN: schedPeek U = Some tid)
         (Htid: containsThread ms tid)
         (Hcmpt: mem_compatible ms m)
-        (Htstep: resume_thread Htid ms'),
+        (Htstep: resume_thread genv m Htid ms'),
         external_step U [::] ms m U [::] ms' m
   | suspend_step':
       forall tid U U' ms ms' m
@@ -326,7 +325,7 @@ Module CoarseMachine (SCH:Scheduler)(SIG : ConcurrentMachineSig with Module Thre
         (HschedS: schedSkip U = U')        (*Schedule Forward*)
         (Htid: containsThread ms tid)
         (Hcmpt: mem_compatible ms m)
-        (Htstep:suspend_thread Htid ms'),
+        (Htstep:suspend_thread genv m Htid ms'),
         external_step U [::] ms m U' [::] ms' m
   | sync_step':
       forall tid U U' ms ms' m m' ev
@@ -368,7 +367,7 @@ Module CoarseMachine (SCH:Scheduler)(SIG : ConcurrentMachineSig with Module Thre
       @internal_step ge U st m st' m' ->
       @machine_step ge U nil st m U nil st' m'.
   Proof. move=>  ge U st m st' m' istp.
-         by inversion istp; econstructor; eauto.
+        inversion istp; try solve [econstructor; eauto].
   Qed.
    Lemma step_equivalence3: forall ge U tr st m U' tr' st' m',
       @external_step ge U tr st m U' tr' st' m' ->
@@ -386,15 +385,15 @@ Module CoarseMachine (SCH:Scheduler)(SIG : ConcurrentMachineSig with Module Thre
 
   Definition MachState: Type := (Sch * event_trace * machine_state)%type.
 
-  Definition MachStep G (c:MachState) (m:mem)
+  Definition MachStep ge (c:MachState) (m:mem)
              (c' :MachState) (m':mem) :=
-    @machine_step G (fst (fst c)) (snd (fst c)) (snd c)  m
+    @machine_step ge (fst (fst c)) (snd (fst c)) (snd c)  m
                   (fst (fst c')) (snd (fst c')) (snd c')  m'.
 
-  Definition at_external (st : MachState)
+  Definition at_external (ge: G) (st : MachState) (m: mem)
     : option (external_function * list val) := None.
 
-  Definition after_external (ov : option val) (st : MachState) :
+  Definition after_external (ge: G) (ov : option val) (st : MachState) :
     option (MachState) := None.
 
   (*not clear what the value of halted should be*)
@@ -412,11 +411,11 @@ Module CoarseMachine (SCH:Scheduler)(SIG : ConcurrentMachineSig with Module Thre
 
 
   Definition init_machine (U:schedule) (r : option RES.res) the_ge
-             (f : val) (args : list val)
-    : option MachState :=
-    match init_mach r the_ge f args with
+             (m: mem) (f : val) (args : list val)
+    : option (MachState * option mem) :=
+    match init_mach r the_ge m f args with
     | None => None
-    | Some c => Some (U, [::], c)
+    | Some (c,m') => Some ((U, [::], c), m')
     end.
 
   Program Definition MachineSemantics (U:schedule) (r : option RES.res):
@@ -434,13 +433,10 @@ Module CoarseMachine (SCH:Scheduler)(SIG : ConcurrentMachineSig with Module Thre
   auto.
   Defined.
 
-  Definition init_machine' (r : option RES.res) the_ge
+  Definition init_machine' (r : option RES.res) the_ge (m: mem)
              (f : val) (args : list val)
-    : option (machine_state) :=
-    match init_mach r the_ge f args with
-    | None => None
-    | Some c => Some (c)
-    end.
+    : option (machine_state * option mem) :=
+    init_mach r the_ge m f args.
 
   (*This is not used anymore:
    * find_thread
@@ -483,11 +479,11 @@ Module CoarseMachine (SCH:Scheduler)(SIG : ConcurrentMachineSig with Module Thre
 
 (*
   Definition MachineSemantics:= MachineSemantics'.*)
-  Lemma initial_schedule: forall genv main vals U U' p c tr n,
-      initial_core (MachineSemantics U p) n genv main vals = Some (U',tr,c) ->
+  Lemma initial_schedule: forall genv m main vals U U' p c tr m' n,
+      initial_core (MachineSemantics U p) n genv m main vals = Some ((U',tr,c),m') ->
       U' = U /\ tr = nil.
         simpl. unfold init_machine. intros.
-        destruct (init_mach p genv main vals); try solve[inversion H].
+        destruct (init_mach p genv m main vals) as [[? ?] |]; try solve[inversion H].
         inversion H; subst; split; auto.
   Qed.
 
@@ -1058,6 +1054,7 @@ Module CoarseMachine (SCH:Scheduler)(SIG : ConcurrentMachineSig with Module Thre
             {core_ord : core_data -> core_data -> Prop}
             (core_ord_wf : well_founded core_ord).
 
+
     Definition stutter_stepN_safety ge cd (U:Sch) (st:machine_state) (m:mem): Prop:=
     @exp_safetyN_stutter _ _ (fun U stm => halted (U, nil, fst stm))
                    (fun U stm stm' => @internal_step ge U (fst stm) (snd stm) (fst stm') (snd stm'))
@@ -1133,65 +1130,65 @@ Module FineMachine (SCH:Scheduler)(SIG : ConcurrentMachineSig with Module Thread
   Notation machine_state := ThreadPool.t.
   Notation event_trace := (seq machine_event).
 
-  Inductive start_thread' genv: forall {tid0} {ms:machine_state},
-      containsThread ms tid0 -> machine_state -> Prop:=
-  | StartThread: forall tid0 ms ms' c_new vf arg
+  Inductive start_thread' genv: forall (m: mem) {tid0} {ms:machine_state},
+      containsThread ms tid0 -> machine_state -> mem -> Prop:=
+  | StartThread: forall m tid0 ms ms' c_new vf arg om
                    (ctn: containsThread ms tid0)
                    (Hcode: getThreadC ctn = Kinit vf arg)
-                   (Hinitial: initial_core Sem (tid2nat tid0) genv vf (arg::nil) = Some c_new)
+                   (Hinitial: initial_core Sem (tid2nat tid0) genv m vf (arg::nil) = Some (c_new, om))
                    (Hinv: invariant ms)
                    (Hms': updThreadC ctn (Krun c_new)  = ms'),
-      start_thread' genv ctn ms'.
-  Definition start_thread genv: forall {tid0 ms},
-      containsThread ms tid0 -> machine_state -> Prop:=
+      start_thread' genv m ctn ms' (option_proj m om).
+  Definition start_thread genv: forall (m: mem) {tid0 ms},
+      containsThread ms tid0 -> machine_state -> mem -> Prop:=
     @start_thread' genv.
 
-  Inductive resume_thread': forall {tid0} {ms:machine_state},
+  Inductive resume_thread' ge: forall (m: mem) {tid0} {ms:machine_state},
       containsThread ms tid0 -> machine_state -> Prop:=
-  | ResumeThread: forall tid0 ms ms' c c' X
+  | ResumeThread: forall m tid0 ms ms' c c' X
                     (ctn: containsThread ms tid0)
-                    (Hat_external: at_external Sem c = Some X)
+                    (Hat_external: at_external Sem ge c m = Some X)
                     (Hafter_external:
-                       after_external Sem None c = Some c')
+                       after_external Sem ge None c = Some c')
                     (Hcode: getThreadC ctn = Kresume c Vundef)
                     (Hinv: invariant ms)
                     (Hms': updThreadC ctn (Krun c')  = ms'),
-      resume_thread' ctn ms'.
-  Definition resume_thread: forall {tid0 ms},
+      resume_thread' ge m ctn ms'.
+  Definition resume_thread ge: forall (m: mem) {tid0 ms},
       containsThread ms tid0 -> machine_state -> Prop:=
-    @resume_thread'.
+    @resume_thread' ge.
 
-  Inductive suspend_thread': forall {tid0} {ms:machine_state},
+  Inductive suspend_thread' ge: forall (m: mem) {tid0} {ms:machine_state},
       containsThread ms tid0 -> machine_state -> Prop:=
-  | SuspendThread: forall tid0 ms ms' c X
+  | SuspendThread: forall m tid0 ms ms' c X
                      (ctn: containsThread ms tid0)
                      (Hcode: getThreadC ctn = Krun c)
-                     (Hat_external: at_external Sem c = Some X)
+                     (Hat_external: at_external Sem ge c m = Some X)
                      (Hinv: invariant ms)
                      (Hms': updThreadC ctn (Kblocked c) = ms'),
-      suspend_thread' ctn ms'.
-  Definition suspend_thread : forall {tid0 ms},
+      suspend_thread' ge m ctn ms'.
+  Definition suspend_thread ge: forall (m: mem) {tid0 ms},
       containsThread ms tid0 -> machine_state -> Prop:=
-    @suspend_thread'.
+    @suspend_thread' ge.
 
   Inductive machine_step {genv:G}:
     Sch -> event_trace -> machine_state -> mem -> Sch
     -> event_trace -> machine_state -> mem -> Prop :=
   | start_step:
-      forall tid U U' ms ms' m tr
+      forall tid U U' ms ms' m m' tr
         (HschedN: schedPeek U = Some tid)
         (HschedS: schedSkip U = U')        (*Schedule Forward*)
         (Htid: containsThread ms tid)
         (Hcmpt: mem_compatible ms m)
-        (Htstep: start_thread genv Htid ms'),
-        machine_step U tr ms m U' tr ms' m
+        (Htstep: start_thread genv m Htid ms' m'),
+        machine_step U tr ms m U' tr ms' m'
   | resume_step:
       forall tid U U' ms ms' m tr
         (HschedN: schedPeek U = Some tid)
         (HschedS: schedSkip U = U')        (*Schedule Forward*)
         (Htid: containsThread ms tid)
         (Hcmpt: mem_compatible ms m)
-        (Htstep: resume_thread Htid ms'),
+        (Htstep: resume_thread genv m Htid ms'),
         machine_step U tr ms m U' tr ms' m
   | thread_step:
       forall tid U U' ms ms' m m' ev tr
@@ -1209,7 +1206,7 @@ Module FineMachine (SCH:Scheduler)(SIG : ConcurrentMachineSig with Module Thread
         (HschedS: schedSkip U = U')        (*Schedule Forward*)
         (Htid: containsThread ms tid)
         (Hcmpt: mem_compatible ms m)
-        (Htstep: suspend_thread Htid ms'),
+        (Htstep: suspend_thread genv m Htid ms'),
         machine_step U tr ms m U' tr ms' m
   | sync_step:
       forall tid U U' ms ms' m m' tr ev
@@ -1244,10 +1241,10 @@ Module FineMachine (SCH:Scheduler)(SIG : ConcurrentMachineSig with Module Thread
     @machine_step G (fst (fst c)) (snd (fst c)) (snd c)  m
                   (fst (fst c')) (snd (fst c')) (snd c')  m'.
 
-  Definition at_external (st : MachState)
+  Definition at_external (ge: G) (st : MachState) (m: mem)
     : option (external_function * list val) := None.
 
-  Definition after_external (ov : option val) (st : MachState) :
+  Definition after_external (ge: G) (ov : option val) (st : MachState) :
     option (MachState) := None.
 
   Definition halted (st : MachState) : option val :=
@@ -1256,11 +1253,11 @@ Module FineMachine (SCH:Scheduler)(SIG : ConcurrentMachineSig with Module Thread
     | _ => Some Vundef
     end.
 
-  Definition init_machine (U:schedule) (p : option RES.res) the_ge
-             (f : val) (args : list val) : option MachState :=
-    match init_mach p the_ge f args with
+  Definition init_machine (U:schedule) (p : option RES.res) the_ge (m: mem)
+             (f : val) (args : list val) : option (MachState * option mem):=
+    match init_mach p the_ge m f args with
     | None => None
-    | Some c => Some (U, [::],c)
+    | Some (c, om) => Some ((U, [::],c), om)
     end.
 
   Program Definition MachineSemantics (U:schedule) (p : option RES.res):
@@ -1279,11 +1276,11 @@ Module FineMachine (SCH:Scheduler)(SIG : ConcurrentMachineSig with Module Thread
   Defined.
 
 
-  Lemma initial_schedule: forall genv main vals U U' p c tr n,
-      initial_core (MachineSemantics U p) n genv main vals =  Some (U',tr,c) ->
+  Lemma initial_schedule: forall genv m main vals U U' p c tr om n,
+      initial_core (MachineSemantics U p) n genv m main vals =  Some ((U',tr,c), om) ->
       U' = U /\ tr = nil.
         simpl. unfold init_machine. intros.
-        destruct (init_mach p genv main vals); try solve[inversion H].
+        destruct (init_mach p genv m main vals) as [[? ?]|]; try solve[inversion H].
         inversion H; subst; split; auto.
   Qed.
 
