concurrency/Asm_core.v
@@ -1,4 +1,5 @@
 Require Import sepcomp.semantics.
+Require Import compcert.lib.Coqlib.
 (* Require Import sepcomp.simulations. *)
 Require Import ZArith List.
 Import ListNotations.
@@ -20,7 +21,6 @@ Definition cl_halted (c: regset) : option val := None.
 
 Definition empty_function : function := 
   mkfunction (mksignature nil None cc_default) nil.
-Check Locations.Outgoing.
 
 Definition get_extcall_arg (inout: Locations.slot) (rs: regset) (m: mem) (l: Locations.loc) : option val :=
  match l with
@@ -162,3 +162,215 @@ Program Definition cl_core_sem :
     cl_step
     cl_corestep_not_at_external
     cl_corestep_not_halted _.
+
+Section ASM_MEMSEM.
+
+Lemma exec_load_mem_step ge ch m a rs rd rs' m': forall
+      (EI: exec_load ge ch m a rs rd = Next rs' m'),
+      mem_step m m'.
+Proof. intros.
+  unfold exec_load in EI.
+  remember (Mem.loadv ch m (eval_addrmode ge a rs) ).
+  symmetry in Heqo; destruct o; inversion EI; clear EI; subst. apply mem_step_refl.
+Qed.
+
+Lemma exec_store_mem_step ge ch m a rs rs0 vals rs' m': forall
+      (ES: exec_store ge ch m a rs rs0 vals = Next rs' m'),
+      mem_step m m'.
+Proof. intros.
+  unfold exec_store in ES.
+  remember (Mem.storev ch m (eval_addrmode ge a rs) (rs rs0)).
+  symmetry in Heqo; destruct o; inversion ES; clear ES; subst.
+  remember (eval_addrmode ge a rs). destruct v; inversion Heqo; clear Heqo; subst.
+  eapply mem_step_store; eassumption.
+Qed.
+
+Lemma goto_label_mem_step c0 l rs m rs' m': forall
+      (G: goto_label c0 l rs m = Next rs' m'),
+      mem_step m m'.
+Proof. intros.
+   unfold goto_label in G.
+   destruct (label_pos l 0 (fn_code c0)); inversion G; clear G; subst.
+   destruct (rs PC); inversion H0; clear H0; subst.
+   apply mem_step_refl.
+Qed.
+
+Lemma exec_instr_mem_step ge c i rs m rs' m': forall
+      (EI: exec_instr ge c i rs m = Next rs' m'),
+      mem_step m m'.
+Proof. intros.
+   destruct i; simpl in *; inversion EI; clear EI; subst; try apply mem_step_refl;
+   try (eapply exec_load_mem_step; eassumption);
+   try (eapply exec_store_mem_step; eassumption).
+
+   destruct (Val.divu (rs EAX) (rs # EDX <- Vundef r1)); inversion H0; clear H0; subst.
+   destruct (Val.modu (rs EAX) (rs # EDX <- Vundef r1)); inversion H1; clear H1; subst.
+   apply mem_step_refl.
+
+   destruct (Val.divs (rs EAX) (rs # EDX <- Vundef r1)); inversion H0; clear H0; subst.
+   destruct (Val.mods (rs EAX) (rs # EDX <- Vundef r1)); inversion H1; clear H1; subst.
+   apply mem_step_refl.
+
+   destruct (eval_testcond c0 rs); inversion H0; clear H0; subst.
+   destruct b; inversion H1; clear H1; subst; apply mem_step_refl.
+   apply mem_step_refl.
+
+   eapply goto_label_mem_step; eassumption.
+
+   destruct (eval_testcond c0 rs); inversion H0; clear H0; subst.
+   destruct b; inversion H1; clear H1; subst.
+   eapply goto_label_mem_step; eassumption.
+   apply mem_step_refl.
+
+   destruct (eval_testcond c1 rs); inversion H0; clear H0; subst.
+   destruct b.
+     destruct (eval_testcond c2 rs); inversion H1; clear H1; subst.
+     destruct b; inversion H0; clear H0; subst.
+     eapply goto_label_mem_step; eassumption.
+   apply mem_step_refl.
+
+     destruct (eval_testcond c2 rs); inversion H1; clear H1; subst.
+     apply mem_step_refl.
+     destruct (rs r); inversion H0; clear H0; subst.
+     destruct (list_nth_z tbl (Int.unsigned i)); inversion H1; clear H1; subst.
+     eapply goto_label_mem_step; eassumption.
+  remember (Mem.alloc m 0 sz) as d; apply eq_sym in Heqd.
+    destruct d; inv H0.
+    remember (Mem.store Mint32 m0 b (Int.unsigned (Int.add Int.zero ofs_link))
+         (rs ESP)) as q.
+    apply eq_sym in Heqq; destruct q; inversion H1; clear H1; subst.
+    remember (Mem.store Mint32 m1 b (Int.unsigned (Int.add Int.zero ofs_ra))
+         (rs RA)) as w.
+    destruct w; apply eq_sym in Heqw; inv H0.
+    eapply mem_step_trans.
+      eapply mem_step_alloc; eassumption.
+    eapply mem_step_trans.
+      eapply mem_step_store; eassumption.
+      eapply mem_step_store; eassumption.
+  destruct (Mem.loadv Mint32 m (Val.add (rs ESP) (Vint ofs_ra))); inv H0.
+    destruct (Mem.loadv Mint32 m (Val.add (rs ESP) (Vint ofs_link))); inv H1.
+    destruct (rs ESP); inv H0.
+    remember (Mem.free m b 0 sz) as t.
+    destruct t; inv H1; apply eq_sym in Heqt.
+    eapply mem_step_free; eassumption.
+Qed.
+
+Lemma asm_mem_step : forall ge c m c' m' (CS: corestep cl_core_sem ge c m c' m'), mem_step m m'.
+Proof. intros.
+  inv CS; simpl in *; try apply mem_step_refl; try contradiction.
++ inv H0. eapply exec_instr_mem_step; try eassumption.
+    clear - H9 H10.
+    admit.
+    admit.
+(*+ eapply extcall_mem_step; eassumption. *)
+(*+ inv H1. eapply extcall_mem_step; try eassumption. apply EFhelpers in OBS; assumption.
+  destruct callee; simpl in *; solve [intros NN; trivial].*)
+Admitted.
+
+Lemma ple_exec_load:
+    forall g ch m a rs rd rs' m'
+       m1 (PLE: perm_lesseq m m1),
+       exec_load g ch m a rs rd = Next rs' m' ->
+       m'=m /\ exec_load g ch m1 a rs rd = Next rs' m1.
+Proof.
+  intros.
+  unfold exec_load in *.
+  destruct (Mem.loadv ch m (eval_addrmode g a rs)) eqn:?; inv H.
+  split; auto.
+  eapply ple_load in Heqo; eauto. rewrite Heqo. auto.
+Qed.
+
+
+Lemma ple_exec_store:
+  forall g ch m a rs rs0 rsx rs' m' m1
+   (PLE: perm_lesseq m m1),
+   exec_store g ch m a rs rs0 rsx = Next rs' m' ->
+  exists m1',
+    perm_lesseq m' m1' /\ exec_store g ch m1 a rs rs0 rsx = Next rs' m1'.
+Proof.
+intros.
+ unfold exec_store in *.
+ destruct (Mem.storev ch m (eval_addrmode g a rs) (rs rs0)) eqn:?; inv H.
+ destruct (ple_store _ _ _ _ _ _ PLE Heqo) as [m1' [? ?]].
+ exists m1'; split; auto.
+ rewrite H0. auto.
+Qed.
+
+Lemma asm_inc_perm: forall (g : genv) c m c' m'
+      (CS:corestep cl_core_sem g c m c' m')
+      m1 (PLE: perm_lesseq m m1),
+      exists m1', corestep cl_core_sem g c m1 c' m1' /\ perm_lesseq m' m1'.
+Proof.
+intros; inv CS; simpl in *; try contradiction.
+inv H0.
++
+assert (cl_at_external g c m1 = None).
+unfold cl_at_external in *. rewrite H5 in *. rewrite H6 in *. auto. 
+ destruct i; simpl in *; inv H8;
+     try solve [
+      exists m1; split; [split | ]; trivial; econstructor; try eassumption; reflexivity
+     | destruct (ple_exec_load _ _ _ _ _ _ _ _ _ PLE H2); subst m';
+        exists m1; split; [split | ]; simpl; auto; econstructor; eassumption
+     | destruct (ple_exec_store _ _ _ _ _ _ _ _ _ _ PLE H2) as [m1' [? ?]];
+        exists m1'; split; [split | ]; auto; econstructor; eassumption
+    |  exists m1; split; [split | ]; auto; [ econstructor; try eassumption; simpl | ];
+       repeat match type of H2 with match ?A with Some _ => _ | None => _ end = _ =>
+         destruct A; try now inv H2 end;
+       eassumption
+    ].
+ - (* Pcmp_rr case fails! *)
+(*+ exists m1; split; trivial. econstructor; try eassumption. admit.
++ admit.
+*)
+Abort.
+
+Program Definition Asm_mem_sem : @MemSem genv regset.
+Proof.
+apply Build_MemSem with (csem := cl_core_sem).
+  apply (asm_mem_step).
+(*  apply asm_inc_perm.*)
+Defined.
+
+Lemma exec_instr_forward g c i rs m rs' m': forall
+      (EI: exec_instr g c i rs m = Next rs' m'),
+      mem_forward m m'.
+Proof. intros.
+    apply mem_forward_preserve.
+    eapply exec_instr_mem_step; eassumption.
+Qed.
+
+End ASM_MEMSEM.
+
+Require Import concurrency.load_frame.
+Lemma load_frame_store_args_rec_nextblock:
+  forall args m m2 stk ofs tys
+    (Hload_frame: store_args_rec m stk ofs args tys = Some m2),
+    Mem.nextblock m2 = Mem.nextblock m.
+Proof.
+  intro args.
+  induction args; intros; simpl in *.
+  destruct tys; inv Hload_frame; auto.
+  destruct tys; try discriminate;
+  destruct t;
+  repeat match goal with
+         | [H: match ?Expr with _ => _ end = _ |- _] =>
+           destruct Expr eqn:?; try discriminate;
+             unfold load_frame.store_stack in *
+         | [H: Mem.storev _ _ _ _ = _ |- _] =>
+           eapply nextblock_storev in H
+         | [H: ?Expr = ?Expr2 |- context[?Expr2]] =>
+           rewrite <- H
+         end;
+  eauto.
+Qed.
+
+Lemma load_frame_store_nextblock:
+  forall m m2 stk args tys
+    (Hload_frame: store_args m stk args tys = Some m2),
+    Mem.nextblock m2 = Mem.nextblock m.
+Proof.
+  intros.
+  unfold load_frame.store_args in *.
+  eapply load_frame_store_args_rec_nextblock; eauto.
+Qed.
+
