concurrency/machine_simulation.v
@@ -45,12 +45,12 @@ Record Machine_sim: Type :=
     
  MSord_wf : well_founded MSorder
 ; core_initial :
-    forall j c1 vals1 m1 vals2 m2,
-    initial_machine Sem1 ge1 main vals1 = Some c1 ->
+    forall j c1 vals1 m1 m1' vals2 m2 m2',
+    initial_machine Sem1 ge1 m1 main vals1 = Some (c1, m1') ->
     exists (*mu*) cd c2,
       (*as_inj mu = j*
-      /\*) initial_machine Sem2 ge2 main vals2 = Some c2
-      /\ MSmatch_states cd j c1 m1 c2 m2
+      /\*) initial_machine Sem2 ge2 m2 main vals2 = Some (c2, m2')
+      /\ MSmatch_states cd j c1 (option_proj m1 m1') c2 (option_proj m2 m2')
 ; MSthread_diagram :
     forall U st1 m1 st1' m1',
     thread_step Sem1 ge1 U st1 m1 st1' m1' ->
